src/examples/Kuiper.ArrayView.Test.EvenOdds3.fst
@@ -41,7 +41,7 @@ instance _cview_strided
 = {
   fits = ();
   cit  = szlt ((len + stride - 1 - offset) / stride);
-  bij  = fin_size_t_bij _;
+  bij  = fin_size_t_bij ((len + stride - 1 - offset) / stride);
   imap = {
     f = (fun (i : szlt ((len + stride - 1 - offset) / stride)) -> i `SZ.mul` stride `SZ.add` offset <: szlt len);
     is_inj = ez;
@@ -56,6 +56,25 @@ instance _cview_even #et (#len : erased nat{SZ.fits len}) : IView.cview (even_vi
 inline_for_extraction noextract
 instance _cview_odd #et (#len : erased nat{SZ.fits len}) : IView.cview (odd_view et len).iview =
   _cview_strided #et #len 2sz 1sz
+
+(* What is happening?!?! Why isn't this obvious? *)
+
+let _wat_even (#len : nat{SZ.fits len}) :
+  Lemma (reveal (_cview_even #u32 #len).bij == fin_size_t_bij ((len + 2 - 1 - 0) / 2))
+        [SMTPat (_cview_even #u32 #len)]
+= admit()
+
+let _wat_odd (#len : nat{SZ.fits len}) :
+  Lemma (reveal (_cview_odd #u32 #len).bij == fin_size_t_bij ((len + 2 - 1 - 1) / 2))
+        [SMTPat (_cview_odd #u32 #len)]
+= admit()
+
+
+let _sanity1 (#len : nat{SZ.fits len}) (x : szlt ((len + 1) / 2)) : Lemma (ci_to_ai (even_view u32 len) x == SZ.v x)
+  = ()
+
+let _sanity2 (#len : nat{SZ.fits len}) (x : szlt (len / 2)) : Lemma (ci_to_ai (odd_view u32 len) x == SZ.v x)
+  = ()
 
 fn foo_even (a : varray (even_view u32 100))
   (#v0 : erased (lseq u32 50))
@@ -79,12 +98,12 @@ fn foo_odd (a : varray (odd_view u32 100))
 
 let vw = sum_aview (even_view u32 100) (odd_view u32 100)
 
-fn test_simpler (a : gpu_array u32 100)
+fn test (a : gpu_array u32 100)
   (#v0 : erased (lseq u32 100))
   preserves gpu
   requires a |-> v0
-  returns u32
-  ensures exists* v1. a |-> v1
+  returns  u32
+  ensures  a |-> v0
 {
   varray_abs' vw a;
   let va = from_array vw a;
@@ -111,3 +130,94 @@ fn test_simpler (a : gpu_array u32 100)
 
   res
 }
+
+
+noextract
+let seq_evens #a (#n : nat)
+  (s : lseq a n)
+  : Tot (lseq a ((n+1)/2))
+=
+  Seq.init ((n+1)/2) fun i -> Seq.index s (2 * i)
+
+noextract
+let seq_odds #a (#n : nat)
+  (s : lseq a n)
+  : Tot (lseq a (n/2))
+=
+  Seq.init (n/2) fun i -> Seq.index s (2 * i + 1)
+
+noextract
+let seq_interleave #a (#n : nat)
+  (s1 : lseq a ((n + 1) / 2))
+  (s2 : lseq a (n / 2))
+  : Tot (lseq a n)
+=
+  Seq.init n fun i ->
+    if i % 2 = 0 then
+      Seq.index s1 (i / 2)
+    else
+      Seq.index s2 ((i-1) / 2)
+
+let merge_lemma #et (#len:nat) (sl : lseq et ((len + 1) / 2)) (sr : lseq et (len / 2))
+  : Lemma (
+            to_seq (sum_aview (even_view et len) (odd_view et len)) (sl, sr)
+            ==
+            seq_interleave sl sr
+  )
+  [SMTPat (to_seq (sum_aview (even_view et len) (odd_view et len)) (sl, sr))]
+= let aux (i : natlt len)
+      : Lemma (to_seq (sum_aview (even_view et len) (odd_view et len)) (sl, sr) @! i
+               ==
+               seq_interleave sl sr @! i)
+  = admit () // flaky
+  in
+  Classical.forall_intro (Classical.move_requires aux);
+  assert (Seq.equal
+              (to_seq (sum_aview (even_view et len) (odd_view et len)) (sl, sr))
+              (seq_interleave sl sr))
+
+// TODO: Find a comfortable way of proving this. The definition of from_seq uses
+// it_of_nat, which uses choice as it is reversing the (surjective) injection
+// and is probably bad for SMT.
+let split_lemma #et (#len:nat) (s : lseq et len)
+  : Lemma (
+            from_seq (sum_aview (even_view et len) (odd_view et len)) s
+            ==
+            (seq_evens s, seq_odds s)
+  )
+  [SMTPat (from_seq (sum_aview (even_view et len) (odd_view et len)) s)]
+= admit()
+
+fn test_write (a : gpu_array u32 100)
+    (#v0 : erased (lseq u32 100))
+    preserves gpu
+    requires a |-> v0
+    ensures  a |-> Seq.upd (Seq.upd v0 20 42ul) 41 43ul
+  {
+    varray_abs' vw a;
+    let va = from_array vw a;
+
+    let vl, vr = varray_split2
+      (even_view u32 100)
+      (odd_view u32 100)
+      (from_array vw a)
+      #_
+      #(from_seq vw v0) // ARGH, why do I have to provide this!?!??! terrible error otherwise
+      ;
+    // Note: that doesn't happen if we use split2_, the ghost version
+
+    varray_write vl 10sz 42ul;
+    varray_write vr 20sz 43ul;
+
+    let va = varray_join2 vl vr;
+
+    varray_concr va;
+
+    rewrite each core va as a;
+
+    with v1.
+      assert (a |-> v1);
+      assert (pure (Seq.equal v1 (Seq.upd (Seq.upd v0 20 42ul) 41 43ul))); // use extensionality
+
+    ()
+  }
